Try using `RBMap` instead, add docstrings
We add a bit of the proof of `Sub_AndEqz_iff_eq_one`.

Is0.lean
@@ -7,23 +7,29 @@ def P: ℕ := 15 * 2^27 + 1
 
 axiom P_prime: Nat.Prime P 
 instance : Fact (Nat.Prime P) := ⟨P_prime⟩
+
+-- A finite field element.
 abbrev Felt := ZMod P
 
+-- A literal, either a finite field element or a constraint.
 inductive Lit where
   | Val : Felt → Lit
   | Constraint : Prop → Lit
 
--- So now we can have duplicate keys if one maps to a felt and the other to a constraint...
+-- A mapping of variable names to values.
+--
+-- Note: we can have duplicate keys if one maps to a felt and the other to a
+-- constraint...
 structure State where
-  felts : Std.HashMap String Felt
-  constraints : Std.HashMap String Prop
+  felts : Std.RBMap String Felt cmp
+  constraints : Std.RBMap String Prop cmp
 
--- We'll definitely need a context, mapping variable names to values.
-
+-- A parametrized expression. In practice, α will be either `Felt` or `Prop`.
 inductive Expression (α : Type) where
   | Literal : α → Expression α
   | Variable : String → Expression α
 
+-- An operation from the cirgen (circuit generation) MLIR dialect.
 inductive Op where
   | Const : Felt → Op
   | True : Op
@@ -37,6 +43,7 @@ inductive Op where
   | AndCond : Prop → Felt → Prop → Op
   | Variable : String → Op
 
+-- Evaluate a circuit operation to get some kind of literal.
 def Op.eval (state : State) (op : Op) : Lit :=
   match op with
   | Const x => .Val x
@@ -50,16 +57,21 @@ def Op.eval (state : State) (op : Op) : Lit :=
     | .Variable name =>  .Constraint ((state.constraints.findD name _root_.True) ∧ x = .Literal 0)
   | _ => .Constraint False
 
+-- Evaluate `op` and assign its value to `name` in the `state` context.
 def Op.assign (state : State) (op : Op) (name : String) : State :=
   match (Op.eval state op) with
   | .Val x => { state with felts := state.felts.insert name x }
   | .Constraint c => { state with constraints := state.constraints.insert name c }
 
+-- An MLIR program in the `cirgen` (circuit generation) dialect.
 inductive Cirgen where
   | Sequence : Cirgen → Cirgen → Cirgen
   | Assign : String → Op → Cirgen
   | Return : String → Cirgen
 
+-- Step through the entirety of a `Cirgen` MLIR program from initial state
+-- `state`, yielding the post-execution state and possibly a constraint
+-- (`Prop`).
 def Cirgen.step (state : State) (program : Cirgen) : State × Option Prop :=
   match program with
   -- We may want to encode the index of the instruction in `State`, and then
@@ -71,19 +83,42 @@ def Cirgen.step (state : State) (program : Cirgen) : State × Option Prop :=
                     | none => Cirgen.step state' b
   | Return name => (state, some $ state.constraints.findD name _root_.True)
 
+-- The result of stepping through a program that generates `(1 - x) = 0`, which
+-- should be equivalent to checking `x = 1`.
 def subAndEqzActual (x : Felt) : State × Option Prop :=
-  Cirgen.step { felts := Std.HashMap.empty, constraints := Std.HashMap.empty }
+  Cirgen.step { felts := Std.RBMap.empty, constraints := Std.RBMap.empty }
     (.Sequence
-      (.Assign "x-1" (Op.Sub x 1))
-      (.Assign "(x-1)=0"
-        (.AndEqz (.Literal _root_.True) (.Variable "x-1"))))
+      (.Sequence
+        (.Assign "x-1" (Op.Sub x 1))
+        (.Assign "(x-1)=0"
+          (.AndEqz (.Literal _root_.True) (.Variable "x-1"))))
+      (.Return "(x-1)=0"))
 
+-- The expected post-execution state after computing `subAndEqzActual`.
 def subAndEqzExpectedState (x : Felt) : State :=
-  { felts := Std.HashMap.ofList [("x-1", x - 1)]
-  , constraints := Std.HashMap.ofList [("(x-1)=0", x - 1 = (0 : Felt))]
+  { felts := Std.RBMap.ofList [("x-1", x - 1)] cmp
+  , constraints := Std.RBMap.ofList [("(x-1)=0", x - 1 = (0 : Felt))] cmp
   }
 
+-- Check that our `(1 - x) = 0` program is equivalent to `x = 1`.
 theorem Sub_AndEqz_iff_eq_one :
   ∀ x : Felt, (subAndEqzActual x).1 = subAndEqzExpectedState x
-    ∧ ((subAndEqzActual x).2 = some c)
-    ∧ (c ↔ x = 1) := by sorry
+    ∧ (((subAndEqzActual x).2 = some c) → (c ↔ x = 1)) := by
+  intros x
+  apply And.intro
+  sorry
+  intros h
+  unfold subAndEqzActual at h
+  rw [Prod.snd] at h
+  unfold Cirgen.step at h
+  unfold Cirgen.step at h
+  unfold Cirgen.step at h
+  unfold Cirgen.step at h
+  simp only at h
+  rw [Option.some_inj] at h
+  rw [← h]
+  clear h
+  apply Iff.intro
+  unfold Op.assign
+  unfold Op.eval
+  simp only [and_false]
